Use a custom map in thunkLang Prim semantics

compiler/backend/thunkLang_primitivesScript.sml
@@ -4,7 +4,7 @@
 
  *)
 open HolKernel Parse boolLib bossLib term_tactic monadsyntax
-     sumTheory;
+     sumTheory listTheory;
 
 val _ = new_theory "thunkLang_primitives";
 
@@ -66,6 +66,17 @@ Definition map_def:
       ys <- map f xs;
       return (y::ys)
     od
+End
+
+Definition result_map_def:
+  result_map f xs =
+    let ys = MAP f xs in
+      if EXISTS ($= (INL Type_error)) ys then
+        INL Type_error
+      else if EXISTS ($= (INL Diverge)) ys then
+        INL Diverge
+      else
+        INR (MAP OUTR ys)
 End
 
 Definition can_def:
@@ -205,6 +216,41 @@ Proof
   \\ Cases_on ‘g h’ \\ fs []
   \\ ‘map f xs = map g xs’ suffices_by simp_tac std_ss []
   \\ first_x_assum irule \\ fs []
+QED
+
+Theorem result_map_INR:
+  result_map f xs = INR res ⇔ map f xs = INR res
+Proof
+  rw [EQ_IMP_THM]
+  \\ gvs [result_map_def, EXISTS_MAP, MAP_MAP_o, combinTheory.o_DEF,
+          CaseEq "bool"]
+  >- (
+    Induct_on ‘xs’ \\ gs [map_def]
+    \\ rw [] \\ gs []
+    \\ Cases_on ‘f h’ \\ gs []
+    \\ Cases_on ‘x’ \\ gs [])
+  \\ pop_assum mp_tac
+  \\ qid_spec_tac ‘res’
+  \\ Induct_on ‘xs’ \\ simp [map_def]
+  \\ rpt gen_tac
+  \\ Cases_on ‘f h’ \\ gs []
+  \\ Cases_on ‘map f xs’ \\ gs []
+QED
+
+Theorem result_map_CONG[defncong]:
+  ∀xs ys f g.
+    xs = ys ∧
+    (∀x. MEM x xs ⇒ f x = g x) ⇒
+      result_map f xs = result_map g ys
+Proof
+  rw [result_map_def, EVERY_MEM, EXISTS_MEM, MEM_MAP, MAP_MAP_o,
+      combinTheory.o_DEF, MAP_EQ_f] \\ gs []
+  \\ TRY (
+    first_assum (irule_at Any)
+    \\ strip_tac \\ gvs []
+    \\ NO_TAC)
+  \\ last_assum (irule_at Any)
+  \\ strip_tac \\ gvs []
 QED
 
 val _ = export_theory ();
